Define Haskell values

common/HaskellValues.v
@@ -4,7 +4,7 @@ Require Import compcert.common.Values. (* C Values and definition of block *)
 
 Definition haskell_int := int64. (* TODO: Should become a parameter *)
 
-Inductive hval : Type :=
+Inductive hval : Type := (* This should be a parameter too *)
 | HSundef : hval
 | HSint : haskell_int -> hval
 | HSsingle : float32 -> hval
@@ -15,6 +15,58 @@ Inductive hval : Type :=
 Definition HStrue: hval := HSint Int64.one.
 Definition HSfalse: hval := HSint Int64.zero.
 
+Definition from_bool (b :bool) : hval :=
+  if b then HStrue else HSfalse.
 
+Module HaskellVal.
+  
+  Definition eq (x y : hval) : {x=y} + {x<>y}.
+  Proof.
+    decide equality.
+    apply Int64.eq_dec.
+    apply Float32.eq_dec.
+    apply Float.eq_dec.
+    apply Ptrofs.eq_dec.
+    apply eq_block.
+  Defined.
+  Global Opaque eq.
 
+  Definition add (v1 v2 : hval) : hval :=
+    match v1, v2 with
+    | HSint n1, HSint n2 => HSint (Int64.add n1 n2)
+    | _, _ => HSundef
+    end. (* TODO: add pointer arithmetic *)
 
+  Definition sub (v1 v2 : hval) : hval :=
+    match v1, v2 with
+    | HSint n1, HSint n2 => HSint (Int64.sub n1 n2)
+    | _, _ => HSundef
+    end. (* TODO: add pointer arithmetic *)
+
+  Definition mul (v1 v2 : hval) : hval :=
+    match v1, v2 with
+    | HSint n1, HSint n2 => HSint (Int64.mul n1 n2)
+    | _, _ => HSundef
+    end.
+
+  Section COMPARISONS.
+
+    Definition cmp_bool (c : comparison) (v1 v2 : hval) : option bool :=
+      match v1, v2 with
+      | HSint n1, HSint n2 => Some (Int64.cmp c n1 n2)
+      | _, _ => None
+      end.
+
+    Definition of_optbool (ob: option bool): hval :=
+      match ob with
+      | Some true => HStrue
+      | Some false => HSfalse
+      | None => HSundef
+      end.
+
+    Definition cmp (c: comparison) (v1 v2: hval): hval :=
+      of_optbool (cmp_bool c v1 v2).
+
+  End COMPARISONS.
+
+End HaskellVal.
